Simpler (?) definitions of coercions

formalization/ctt.v
@@ -4,81 +4,96 @@ Require itt.
 
 
 (* Coercions between contexts. *)
-Structure contextCoercion {G D : itt.context} :=
-  { ctx_bij : itt.substitution
-  ; ctx_inv : itt.substitution
-  ; ctx_bij_ty : itt.issubst ctx_bij G D
-  ; ctx_inv_ty : itt.issubst ctx_inv D G
-  ; ctx_coh :
-      forall A u,
-        itt.isterm D u A ->
-        { p : itt.term
-        & itt.isterm D p (itt.Id A (itt.subst (itt.subst u ctx_bij) ctx_inv) u)
-        }
+Structure contextCoercion :=
+  { ctxco_map : itt.substitution
+  ; ctxco_inv : itt.substitution
   }.
 
+Definition isContextCoercion c G D := (
+  itt.issubst (ctxco_map c) G D *
+  itt.issubst (ctxco_inv c) D G *
+  (forall A u,
+     itt.isterm D u A ->
+     { p : itt.term
+     & itt.isterm D
+                  p
+                  (itt.Id A
+                          (itt.subst (itt.subst u (ctxco_map c)) (ctxco_inv c))
+                          u
+                  )
+     }
+  ))%type.
+
 (* Coercions between types, over a context coercion. *)
-Structure typeCoercion {G D : itt.context} (c : @contextCoercion G D)
-                       (A B : itt.type) :=
-  { ty_bij : itt.term
-  ; ty_inv : itt.term
-  ; ty_bij_ty :
-      itt.isterm G
-                 ty_bij
-                 (itt.Prod
-                    A
-                    (itt.Subst (itt.Subst B (ctx_bij c)) (itt.sbweak G A)))
-  ; ty_inv_ty :
-      itt.isterm D
-                 ty_inv
-                 (itt.Prod
-                    B
-                    (itt.Subst (itt.Subst A (ctx_inv c)) (itt.sbweak D B)))
-  ; ty_coh :
-      forall x,
+Structure typeCoercion :=
+  { tyco_map : itt.term
+  ; tyco_inv : itt.term
+  }.
+
+(* Type coercion tc is a valid coercion from A to B
+   over context coercion cc from G to D. *)
+Definition istypeCoercion cc G D tc A B :=
+(
+  itt.isterm G
+             (tyco_map tc)
+             (itt.Prod
+                A
+                (itt.Subst (itt.Subst B (ctxco_map cc)) (itt.sbweak G A))) *
+  itt.isterm D
+             (tyco_inv tc)
+             (itt.Prod
+                B
+                (itt.Subst (itt.Subst A (ctxco_inv cc)) (itt.sbweak D B))) *
+  (forall x,
         itt.isterm G x A ->
         { p : itt.term
         & itt.isterm G p
-                     (itt.Id A
-                       (itt.app
-                          (itt.subst ty_inv (ctx_bij c))
-                          (itt.Subst B (ctx_bij c))
-                          (itt.Subst A (itt.sbweak G (itt.Subst B (ctx_bij c))))
-                          (itt.app
-                             ty_bij
-                             A
-                             (itt.Subst (itt.Subst B (ctx_bij c))
-                                        (itt.sbweak G A))
-                             x))
-                       x)
+                     (itt.Id
+                        A
+                        (itt.app
+                           (itt.subst (tyco_inv tc) (ctxco_map cc))
+                           (itt.Subst B (ctxco_map cc))
+                           (itt.Subst
+                              A
+                              (itt.sbweak G (itt.Subst B (ctxco_map cc))))
+                           (itt.app
+                              (tyco_map tc)
+                              A
+                              (itt.Subst (itt.Subst B (ctxco_map cc))
+                                         (itt.sbweak G A))
+                              x))
+                        x)
         }
-  }.
+  )
+)%type.
 
 (* Coercion for a type *)
-Structure typeCoerce : Type :=
-  { ctx_fro : itt.context ;
-    ctx_to  : itt.context ;
-    ctx_co  : @contextCoercion ctx_fro ctx_to
-  }.
+Definition typeCoerce : Type := contextCoercion.
 
 (* Coercion for a term *)
-Structure termCoerce : Type :=
-  { (* ctx_fro : itt.context ; *)
-    (* ctx_to  : itt.context ; *)
-    (* ctx_co  : @contextCoercion ctx_fro ctx_to ; *)
-    full_ctx_co : typeCoerce ; (* Maybe abstract it away? *)
-    ty_fro      : itt.type ;
-    ty_to       : itt.type ;
-    ty_co       : @typeCoercion (ctx_fro full_ctx_co)
-                                (ctx_to  full_ctx_co)
-                                (ctx_co  full_ctx_co)
-                                ty_fro ty_to
-  }.
+Definition termCoerce : Type :=
+  contextCoercion * typeCoercion.
+
+(* Structure termCoerce : Type := *)
+(*   { (* ctx_fro : itt.context ; *) *)
+(*     (* ctx_to  : itt.context ; *) *)
+(*     (* ctx_co  : @contextCoercion ctx_fro ctx_to ; *) *)
+(*     full_ctx_co : typeCoerce ; (* Maybe abstract it away? *) *)
+(*     ty_fro      : itt.type ; *)
+(*     ty_to       : itt.type ; *)
+(*     ty_co       : @typeCoercion (ctx_fro full_ctx_co) *)
+(*                                 (ctx_to  full_ctx_co) *)
+(*                                 (ctx_co  full_ctx_co) *)
+(*                                 ty_fro ty_to *)
+(*   }. *)
 
 Parameter substCoerce : Type.
 
+Definition idTy G : typeCoerce :=
+  {| ctxco_map := itt.sbid G
+   ; ctxco_inv := itt.sbid G |}.
+
 (* These will require parameters. *)
-Parameter idTy : typeCoerce.
 Parameter idTm : termCoerce.
 Parameter idSb : substCoerce.
 
